IIO.Effect.fst
@@ -1,0 +1,125 @@
+module IIO.Effect
+
+open FStar.Tactics
+open ExtraTactics
+
+open Common
+open IO.Free
+open IO.Effect
+
+let rec iio_interpretation #a
+  (m : iio a) 
+  (h : events_trace)
+  (p : io_post a) : Type0 = 
+  match m with
+  | Return x -> p (Inl x) []
+  | Throw err -> p (Inr err) []
+  | Cont (Call GetTrace args fnc) -> (
+      FStar.WellFounded.axiom1 fnc (Inl h);
+      iio_interpretation (fnc (Inl h)) h p
+  )
+  | Cont (Call cmd args fnc) -> (
+    forall res. (
+      FStar.WellFounded.axiom1 fnc res;
+      let event : io_event = convert_call_to_event cmd args res in
+      iio_interpretation (fnc res) (event::h) (gen_post p event)))
+
+
+// REFINED COMPUTATION MONAD (repr)
+let irepr (a:Type) (wp:io_wpty a) =
+  h:events_trace -> post:io_post a ->
+    Pure (iio a)
+      (requires (wp h post))
+      (ensures (fun (t:iio a) -> iio_interpretation t h post))
+
+let ireturn (a : Type) (x : a) : irepr a (io_return_wp a x) =
+  fun _ _ -> iio_return a x
+
+let w = io_wpty
+
+unfold
+val w_ord (#a : Type) : w a -> w a -> Type0
+let w_ord wp1 wp2 = forall h p. wp1 h p ==> wp2 h p
+
+let ibind (a b : Type) (wp_v : w a) (wp_f: a -> w b) (v : irepr a wp_v)
+  (f : (x:a -> irepr b (wp_f x))) : irepr b (io_bind_wp _ _ wp_v wp_f) =
+  fun h p -> 
+    let t = (iio_bind a b 
+        (v h (compute_post a b h wp_f p))
+        (fun x ->
+          assume (wp_f x h p);
+           f x h p)) in
+    assume (iio_interpretation t h p);
+    t
+
+unfold
+let isubcomp (a:Type) (wp1 wp2: w a) (f : irepr a wp1) :
+  Pure (irepr a wp2) (requires w_ord wp2 wp1) (ensures fun _ -> True) = f
+
+unfold
+let wp_if_then_else (#a:Type) (wp1 wp2:w a) (b:bool) : w a =
+  fun h p -> (b ==> wp1 h p) /\ ((~b) ==> wp2 h p)
+
+unfold
+let i_if_then_else (a : Type) (wp1 wp2 : w a) (f : irepr a wp1) (g : irepr a wp2) (b : bool) : Type =
+  irepr a (wp_if_then_else wp1 wp2 b)
+
+total
+reifiable
+reflectable
+layered_effect {
+  IIOwp : a:Type -> wp : io_wpty a -> Effect
+  with
+       repr       = irepr
+     ; return     = ireturn
+     ; bind       = ibind
+
+     ; subcomp      = isubcomp
+     ; if_then_else = i_if_then_else
+}
+
+let lift_pure_iiowp (a:Type) (wp:pure_wp a) (f:(eqtype_as_type unit -> PURE a wp)) :
+  Pure (irepr a (fun s0 p -> wp (fun r -> p (Inl r) []))) (requires True)
+                    (ensures (fun _ -> True))
+  = fun s0 p -> let r = elim_pure f (fun r -> p (Inl r) []) in iio_return _ r
+
+sub_effect PURE ~> IOwp = lift_pure_iowp
+
+let lift_iowp_iiowp (a:Type) (wp:io_wpty a) (f:IO.Effect.irepr a wp) :
+  Pure (irepr a (fun s0 p -> wp s0 (fun r le -> p r le))) 
+    (requires True)
+    (ensures (fun _ -> True))
+  // TODO: lift from IO.irepr to IIO.irepr
+  = fun s0 p -> admit (); f s0 p
+
+sub_effect IOwp ~> IIOwp = lift_iowp_iiowp
+  
+effect IIO
+  (a:Type)
+  (pre : events_trace -> Type0)
+  (post : events_trace -> maybe a -> events_trace -> Type0) =
+  IIOwp a (fun (h:events_trace) (p:io_post a) ->
+    pre h /\ (forall res le. post h res le ==>  p res le))
+
+let openfile = static_cmd Openfile
+let read = static_cmd Read
+let close = static_cmd Close
+
+let testStat2 () : 
+  IIO unit (fun h -> True) (fun h _ le -> enforced_locally default_check h le) =
+  let fd = openfile "../Makefile" in
+  let msg = read fd in
+  close fd;
+  ()
+
+let get () : IIO events_trace (fun h -> True) 
+  (fun h r le -> r == (Inl h)) by (
+  let h = forall_intro () in
+  let p = forall_intro () in
+  norm [delta_only[`%iio_interpretation]];
+  let _ = forall_intro () in
+  let g = implies_intro () in
+  let l1, l2 = Tactics.destruct_and g in
+  dump "h") =
+  IIOwp?.reflect (fun _ _ -> iio_all GetTrace ())
+
